Hoare

src/lowparse/LowParse.Spec.Fold.fst
@@ -39,89 +39,125 @@ let rec parser_of_typ (t: typ) : Tot (parser pkind (type_of_typ t)) =
     weaken _ (parse_vldata 1 (parse_list (parser_of_typ t')))
   | TChoice f -> weaken _ (parse_dtuple2 parse_bool (fun x -> parser_of_typ (f x)))
 
-let stt (state_t: Type) (ret_t: Type) : Tot Type = state_t -> (ret_t & state_t)
+let stt (state_t: Type) (ret_t: Type) (pre: state_t -> prop) (post: state_t -> ret_t -> state_t -> prop) : Tot Type = (x: state_t) -> Pure (ret_t & state_t)
+  (pre x)
+  (fun (r, y) -> post x r y)
 
-let ret (#state_t: Type) (#ret_t: Type) (x: ret_t) : Tot (stt state_t ret_t) = fun s -> (x, s)
+let ret (#state_t: Type) (#ret_t: Type) (x: ret_t) : Tot (stt state_t ret_t (fun _ -> True) (fun s x' s' -> s == s' /\ x == x')) = fun s -> (x, s)
 
-let bind (#state_t: Type) (#ret1_t #ret2_t: Type) (f1: stt state_t ret1_t) (f2: ret1_t -> stt state_t ret2_t) : Tot (stt state_t ret2_t) =
-  fun state ->
-    let (r, state) = f1 state in
-    f2 r state
+let bind (#state_t: Type) (#ret1_t #ret2_t: Type)
+  (#pre1: state_t -> prop)
+  (#post1: state_t -> ret1_t -> state_t -> prop)
+  (f1: stt state_t ret1_t pre1 post1)
+  (#pre2: state_t -> prop)
+  (#post2: state_t -> ret2_t -> state_t -> prop)
+  (f2: (r1: ret1_t) -> stt state_t ret2_t pre2 post2)
+: Pure (stt state_t ret2_t pre1 (fun s0 r2 s2 -> exists r1 s1 .
+    post1 s0 r1 s1 /\
+    pre2 s1 /\
+    post2 s1 r2 s2
+  ))
+  (requires (forall s0 r1 s1 . post1 s0 r1 s1 ==> pre2 s1))
+  (ensures (fun _ -> True))
+= fun state0 ->
+    let (r1, state1) = f1 state0 in
+    let (r2, state2) = f2 r1 state1 in
+    (r2, state2)
 
-let fold_t (state_t: Type) (t: Type) : Tot Type = (t -> stt state_t unit)
+let weaken (#state_t: Type) (pre: state_t -> prop) (post: state_t -> prop) : Pure (stt state_t unit pre (fun _ _ -> post)) (requires (forall s . pre s ==> post s)) (ensures (fun _ -> True)) =
+  fun s -> ((), s)
+
+let fold_t (state_t: Type) (pre post: state_t -> prop) (t: Type) : Tot Type = (t -> stt state_t unit pre (fun _ _ -> post))
 
 let fold_pair
   (#state_t: Type)
+  (#pre1 #post1 #pre2 #post2: state_t -> prop)
   (#t1 #t2: Type)
-  (f1: fold_t state_t t1)
-  (f2: fold_t state_t t2)
-: Tot (fold_t state_t (t1 & t2))
+  (f1: fold_t state_t pre1 post1 t1)
+  (f2: fold_t state_t pre2 post2 t2)
+: Pure (fold_t state_t pre1 post2 (t1 & t2))
+    (requires (forall s . post1 s ==> pre2 s))
+    (ensures (fun _ -> True))
 = fun (x1, x2) -> bind (f1 x1) (fun _ -> f2 x2)
 
 let fold_list
   (#state_t: Type)
+  (#inv: state_t -> prop)
   (#t: Type)
-  (f: fold_t state_t t)
-: Tot (fold_t state_t (list t))
-= fun l x -> ((), List.Tot.fold_left (fun state x -> snd (f x state)) x l)
+  (f: fold_t state_t inv inv t)
+: Tot (fold_t state_t inv inv (list t))
+= fun l x -> ((), (List.Tot.fold_left (fun (state: state_t { inv state }) x -> snd (f x state)) x l <: state_t))
 
 let fold_choice
   (#state_t: Type)
+  (#pre #post: state_t -> prop)
   (#t: bool -> Type)
-  (f: (x: bool) -> fold_t state_t (t x))
-: Tot (fold_t state_t (x: bool & t x))
+  (f: (x: bool) -> fold_t state_t pre post (t x))
+: Tot (fold_t state_t pre post (x: bool & t x))
 = fun w -> if (dfst w) then f true (dsnd w) else f false (dsnd w)
 
 let bind_fold
   (#state_t: Type)
   (#ret_t: Type)
+  (#pre1: _)
+  (#post1: _)
+  (#pre2 #post2: _)
   (#t: Type)
-  (f: stt state_t ret_t)
-  (g: ret_t -> fold_t state_t t)
-: Tot (fold_t state_t t)
+  (f: stt state_t ret_t pre1 post1)
+  (g: ret_t -> fold_t state_t pre2 post2 t)
+: Pure (fold_t state_t pre1 post2 t)
+    (requires (forall s r s' . post1 s r s' ==> pre2 s'))
+    (ensures (fun _ -> True))
 = fun x -> bind f (fun r -> g r x)
 
 let seq_fold
   (#state_t: Type)
+  (#pre1 #post1 #pre2 #post2: _)
   (#t: Type)
-  (f1 f2: fold_t state_t t)
-: Tot (fold_t state_t t)
+  (f1: fold_t state_t pre1 post1 t)
+  (f2: fold_t state_t pre2 post2 t)
+: Pure (fold_t state_t pre1 post2 t)
+    (requires (forall s . post1 s ==> pre2 s))
+    (ensures (fun _ -> True))
 = fun x -> bind (f1 x) (fun _ -> f2 x)
 
 let ret_fold
   (#state_t: Type)
+  (#pre #post: _)
   (#t: Type)
-  (f: stt state_t unit)
-: Tot (fold_t state_t t)
+  (f: stt state_t unit pre (fun _ _ -> post))
+: Tot (fold_t state_t pre post t)
 = fun _ -> f
 
 noeq
 type prog
   (state_t: Type)
-  (action_t: (t: Type) -> stt state_t t -> Type)
-: typ -> Type
-= | PRet: (t: typ) -> (s: stt state_t unit) -> action_t _ s -> prog state_t action_t t
-  | PSeq: (#t: typ) -> prog state_t action_t t -> prog state_t action_t t -> prog state_t action_t t
-  | PBind: (#r: Type) -> (#t: typ) -> (s: stt state_t r) -> action_t r s -> (r -> prog state_t action_t t) -> prog state_t action_t t
-  | PU8: (s: (U8.t -> stt state_t unit)) -> ((x: U8.t) -> action_t _ (s x)) -> prog state_t action_t TU8
-  | PPair: (#t1: typ) -> (#t2: typ) -> prog state_t action_t t1 -> prog state_t action_t t2 -> prog state_t action_t (TPair t1 t2)
-  | PList: (#t: typ) -> prog state_t action_t t -> prog state_t action_t (TList t)
-  | PChoice: (f: (bool -> typ)) -> ((x: bool) -> prog state_t action_t (f x)) -> prog state_t action_t (TChoice f)
+  (action_t: (t: Type) -> (pre: _) -> (post: _) -> stt state_t t pre post -> Type)
+: (state_t -> prop) -> (state_t -> prop) -> typ -> Type
+= | PRet: (#pre: _) -> (#post: _) -> (t: typ) -> (s: stt state_t unit pre (fun _ _ -> post)) -> action_t _ pre (fun _ _ -> post) s -> prog state_t action_t pre post t
+  | PSeq: (#t: typ) -> (#pre1: _) -> (#post1: (_ -> prop)) -> (#pre2: (_ -> prop)  { forall s . post1 s ==> pre2 s }) -> (#post2: _) -> prog state_t action_t pre1 post1 t -> prog state_t action_t pre2 post2 t -> prog state_t action_t pre1 post2 t
+  | PBind: (#r: Type) -> (#pre1: _) -> (#post1: (_ -> _ -> _ -> prop)) -> (#pre2: (_ -> prop) { forall s0 r1 s1 . post1 s0 r1 s1 ==> pre2 s1 }) -> (#post2: _) -> (#t: typ) -> (s: stt state_t r pre1 post1) -> action_t r pre1 post1 s -> (r -> prog state_t action_t pre2 post2 t) -> prog state_t action_t pre1 post2 t
+  | PU8: (#pre: _) -> (#post: _) -> (s: (U8.t -> stt state_t unit pre (fun _ _ -> post))) -> ((x: U8.t) -> action_t _ _ _ (s x)) -> prog state_t action_t pre post TU8
+  | PPair: (#t1: typ) -> (#t2: typ) -> (#pre1: _) -> (#post1: (_ -> prop)) -> (#pre2: (_ -> prop) { forall s . post1 s ==> pre2 s }) -> (#post2: _) -> prog state_t action_t pre1 post1 t1 -> prog state_t action_t pre2 post2 t2 -> prog state_t action_t pre1 post2 (TPair t1 t2)
+  | PList: (#t: typ) -> (#inv: _) -> prog state_t action_t inv inv t -> prog state_t action_t inv inv (TList t)
+  | PChoice: (f: (bool -> typ)) -> (#pre: _) -> (#post: _) -> ((x: bool) -> prog state_t action_t pre post (f x)) -> prog state_t action_t pre post (TChoice f)
 
 let rec sem
   (#state_t: Type)
-  (#action_t: (t: Type) -> stt state_t t -> Type)
+  (#action_t: (t: Type) -> (pre: _) -> (post: _) -> stt state_t t pre post -> Type)
+  (#pre: _)
+  (#post: _)
   (#t: typ)
-  (p: prog state_t action_t t)
-: Tot (fold_t state_t (type_of_typ t))
-= match p returns fold_t state_t (type_of_typ t) with
+  (p: prog state_t action_t pre post t)
+: Tot (fold_t state_t pre post (type_of_typ t))
+= match p returns fold_t state_t pre post (type_of_typ t) with
   | PRet _ s _ -> ret_fold s
   | PSeq p1 p2 -> seq_fold (sem p1) (sem p2)
   | PBind s _ p -> bind_fold s (fun x -> sem (p x))
   | PU8 s _ -> s
   | PPair p1 p2 -> fold_pair (sem p1) (sem p2)
   | PList p -> fold_list (sem p)
-  | PChoice f p -> fold_choice (fun x -> sem (p x)) <: fold_t state_t (type_of_typ (TChoice f))
+  | PChoice f p -> fold_choice (fun x -> sem (p x)) <: fold_t state_t pre post (type_of_typ (TChoice f))
 
 (* Step-by-step serialization *)
 
